Refinery/Ctx/Split.lean
@@ -5,11 +5,156 @@ namespace Refinery
 variable [HasQuant α]
 
 inductive Var?.Split : Var? α → Var? α → Var? α → Type _
-  | left {v w} (h : v ≤ w) : Split v w v.erase
-  | right {v w} (h : v ≤ w) : Split v v.erase w
-  | sboth {u v w} : u.scopy → u ≤ v → u ≤ w → Split u v w
+  | neither {A q} : del ⟨A, q⟩ → Split ⟨A, q⟩ ⟨A, 0⟩ ⟨A, 0⟩
+  | left (A q) : Split ⟨A, q⟩ ⟨A, q⟩ ⟨A, 0⟩
+  | right (A q) : Split ⟨A, q⟩ ⟨A, 0⟩ ⟨A, q⟩
+  | both {u} : u.copy → Split u u u
+
+abbrev Var?.splitN (v : Var? α) [hv : v.del] : v.Split v.erase v.erase := .neither hv
+
+abbrev Var?.splitL (v : Var? α) : v.Split v v.erase := .left v.ty v.q
+
+abbrev Var?.splitR (v : Var? α) : v.Split v.erase v := .right v.ty v.q
+
+abbrev Var?.splitB (v : Var? α) [hv : v.copy] : v.Split v v := .both hv
+
+theorem Var?.Split.left_unused {u v w : Var? α} (σ : u.Split v w) (h : u.unused) : v.unused
+  := by cases σ <;> first | assumption | rfl
+
+theorem Var?.Split.right_unused {u v w : Var? α} (σ : u.Split v w) (h : u.unused) : w.unused
+  := by cases σ <;> first | rfl | assumption
+
+theorem Var?.Split.used_of_left {u v w : Var? α} (σ : u.Split v w) (h : v.used) : u.used
+  := by cases σ <;> first | assumption | cases h
+
+theorem Var?.Split.used_of_right {u v w : Var? α} (σ : u.Split v w) (h : w.used) : u.used
+  := by cases σ <;> first | cases h | assumption
+
+theorem Var?.Split.erase_eq_left {u v w : Var? α} (h : u.Split v w)
+  : u.erase = v.erase := by cases h <;> simp [*]
+
+theorem Var?.Split.erase_eq_right {u v w : Var? α} (h : u.Split v w)
+  : u.erase = w.erase := by cases h <;> simp [*]
+
+theorem Var?.Split.erase_eq_both {u v w : Var? α} (h : u.Split v w)
+  : v.erase = w.erase := by cases h <;> simp [*]
 
 inductive Ctx?.Split : Ctx? α → Ctx? α → Ctx? α → Type _ where
   | nil : Ctx?.Split .nil .nil .nil
   | cons {Γ Δ Ξ v l r} (h : Split Γ Δ Ξ) (hvw : v.Split l r)
     : Split (Ctx?.cons Γ v) (Ctx?.cons Δ l) (Ctx?.cons Ξ r)
+
+def Var?.Split.hasLeft {u v w : Var? α} : u.Split v w → Bool
+  | .left _ _ => true | .both _ => true | _ => false
+
+@[simp]
+theorem Var?.Split.hasLeft_neither {A q} [hA : Var?.del ⟨A, q⟩]
+  : (Split.neither (α := α) hA).hasLeft = false := rfl
+
+@[simp]
+theorem Var?.Split.hasLeft_left {A q} : (Split.left (α := α) A q).hasLeft = true := rfl
+
+@[simp]
+theorem Var?.Split.hasLeft_right {A q} : (Split.right (α := α) A q).hasLeft = false := rfl
+
+@[simp]
+theorem Var?.Split.hasLeft_both {u : Var? α} [hu : u.copy] : (Split.both hu).hasLeft = true := rfl
+
+def Var?.Split.hasRight {u v w : Var? α} : u.Split v w → Bool
+  | .right _ _ => true | .both _ => true | _ => false
+
+@[simp]
+theorem Var?.Split.hasRight_neither {A q} [hA : Var?.del ⟨A, q⟩]
+  : (Split.neither (α := α) hA).hasRight = false := rfl
+
+@[simp]
+theorem Var?.Split.hasRight_left {A q} : (Split.left (α := α) A q).hasRight = false := rfl
+
+@[simp]
+theorem Var?.Split.hasRight_right {A q} : (Split.right (α := α) A q).hasRight = true := rfl
+
+@[simp]
+theorem Var?.Split.hasRight_both {u : Var? α} [hu : u.copy] : (Split.both hu).hasRight = true := rfl
+
+def Var?.Split.wkLeft {u v w : Var? α} (u' : Var? α) (σ : u.Split v w) : Var? α
+  := if u.used && σ.hasLeft then u' else u'.erase
+
+def Var?.Split.wkRight {u v w : Var? α} (u' : Var? α) (σ : u.Split v w) : Var? α
+  := if u.used && σ.hasRight then u' else u'.erase
+
+@[simp]
+theorem Var?.Split.wkLeft_neither {u' : Var? α} (A q) [hA : Var?.del ⟨A, q⟩]
+  : (Split.neither hA).wkLeft u' = u'.erase := by simp [wkLeft]
+
+@[simp]
+theorem Var?.Split.wkLeft_left {u' : Var? α} (A q) :
+  (Split.left A q).wkLeft u' = if 1 ≤ q then u' else u'.erase := by simp [wkLeft]
+
+@[simp]
+theorem Var?.Split.wkLeft_right {u' : Var? α} (A q) :
+  (Split.right A q).wkLeft u' = u'.erase := by simp [wkLeft]
+
+@[simp]
+theorem Var?.Split.wkLeft_both {u' : Var? α} (u : Var? α) [hu : u.copy] :
+  (Split.both hu).wkLeft u' = if u.used then u' else u'.erase := by simp [wkLeft]
+
+@[simp]
+theorem Var?.Split.wkRight_neither {u' : Var? α} (A q) [hA : Var?.del ⟨A, q⟩]
+  : (Split.neither hA).wkRight u' = u'.erase := by simp [wkRight]
+
+@[simp]
+theorem Var?.Split.wkRight_left {u' : Var? α} (A q) :
+  (Split.left A q).wkRight u' = u'.erase := by simp [wkRight]
+
+@[simp]
+theorem Var?.Split.wkRight_right {u' : Var? α} (A q) :
+  (Split.right A q).wkRight u' = if 1 ≤ q then u' else u'.erase := by simp [wkRight]
+
+@[simp]
+theorem Var?.Split.wkRight_both {u' : Var? α} (u : Var? α) [hu : u.copy] :
+  (Split.both hu).wkRight u' = if u.used then u' else u'.erase := by simp [wkRight]
+
+@[simp]
+theorem Var?.Split.wkLeft_unused {u' u v w : Var? α} (σ : u.Split v w) (hu : u.unused) :
+  σ.wkLeft u' = u'.erase := by cases u; cases hu; rfl
+
+@[simp]
+theorem Var?.Split.wkRight_unused {u' u v w : Var? α} (σ : u.Split v w) (hu : u.unused) :
+  σ.wkRight u' = u'.erase := by cases u; cases hu; rfl
+
+@[simp]
+theorem Var?.Split.wkLeft_used {u' u v w : Var? α} (σ : u.Split v w) (hu : u.used) :
+  σ.wkLeft u' = if σ.hasLeft then u' else u'.erase := by rw [wkLeft]; simp [*]
+
+@[simp]
+instance Var?.Split.wkLeft_del {u' u v w : Var? α} [hv : v.del] (ρ : u' ≤ u) (σ : u.Split v w)
+  : (σ.wkLeft u').del := by cases u with | mk A q => cases q using EQuant.casesZero with
+  | zero => simp
+  | rest => cases σ <;> simp [wkLeft] <;> apply Var?.del.anti ρ
+
+@[simp]
+instance Var?.Split.wkLeft_copy {u' u v w : Var? α} [hv : v.copy] (ρ : u' ≤ u) (σ : u.Split v w)
+  : (σ.wkLeft u').copy := by cases u with | mk A q => cases q using EQuant.casesZero with
+  | zero => simp
+  | rest => cases σ <;> simp [wkLeft] <;> apply Var?.copy.anti ρ (by simp)
+
+@[simp]
+instance Var?.Split.wkRight_del {u' u v w : Var? α} [hw : w.del] (ρ : u' ≤ u) (σ : u.Split v w)
+  : (σ.wkRight u').del := by cases u with | mk A q => cases q using EQuant.casesZero with
+  | zero => simp
+  | rest => cases σ <;> simp [wkRight] <;> apply Var?.del.anti ρ
+
+@[simp]
+instance Var?.Split.wkRight_copy {u' u v w : Var? α} [hw : w.copy] (ρ : u' ≤ u) (σ : u.Split v w)
+  : (σ.wkRight u').copy := by cases u with | mk A q => cases q using EQuant.casesZero with
+  | zero => simp
+  | rest => cases σ <;> simp [wkRight] <;> apply Var?.copy.anti ρ (by simp)
+
+def Var?.Split.wk {u' u v w : Var? α} (ρ : u' ≤ u) (σ : u.Split v w) :
+  u'.Split (σ.wkLeft u') (σ.wkRight u') := match u with
+  | ⟨A, 0⟩ => .neither (Var?.del.anti ρ)
+  | ⟨A, (q : Quant)⟩ => match σ with
+    | .neither h => .neither (Var?.del.anti ρ)
+    | .left _ _ => .left _ _
+    | .right _ _ => .right _ _
+    | .both h => .both (Var?.copy.anti ρ (by simp))
